@prefix : <http://neo4j.com/voc/art#> .
@prefix owl: <http://www.w3.org/2002/07/owl#> .
@prefix rdf: <http://www.w3.org/1999/02/22-rdf-syntax-ns#> .
@prefix xml: <http://www.w3.org/XML/1998/namespace> .
@prefix xsd: <http://www.w3.org/2001/XMLSchema#> .
@prefix rdfs: <http://www.w3.org/2000/01/rdf-schema#> .
@base <http://neo4j.com/voc/art#> .

<http://neo4j.com/voc/art#> rdf:type owl:Ontology ;
                             owl:imports <https://schema.org/version/latest/schemaorg-current-https.ttl> .

#################################################################
#    properties
#################################################################

###  http://neo4j.com/voc/art#artworkKnownAs
:artworkKnownAs rdf:type owl:DatatypeProperty , owl:InverseFunctionalProperty ;
                rdfs:comment "represent the title or an identifying description of the artwork" ;
                rdfs:subPropertyOf <https://schema.org/name> ;
                rdfs:range xsd:string ;
                rdfs:domain :Artwork .


###  http://neo4j.com/voc/art#influences
:influences rdf:type owl:ObjectProperty ;
            rdfs:comment "connects an Artist to another Artist indicating that the former is an artistic influence to the later" ;
            rdfs:range :Artist ;
            rdfs:domain :Artist .


###  http://neo4j.com/voc/art#professionalName
:professionalName rdf:type owl:DatatypeProperty , owl:InverseFunctionalProperty ;
                  rdfs:comment "the name used to refer to an artist. May not always match their real name, can be a pseudonym." ;
                  rdfs:subPropertyOf <https://schema.org/name> ;
                  rdfs:range xsd:string ;
                  rdfs:domain :Artist .


###  http://neo4j.com/voc/art#represents
:represents rdf:type owl:ObjectProperty ;
            rdfs:comment "connects an Artwork with something depicted in it" ;
            rdfs:range <https://schema.org/Person> ;
            rdfs:domain :Artwork .


###  http://neo4j.com/voc/art#was_created_by
:was_created_by rdf:type owl:ObjectProperty ;
                rdfs:comment "connects an Artwork to the Artist that is its author" ;
                rdfs:subPropertyOf <https://schema.org/creator> ;
                rdfs:range :Artist ;
                rdfs:domain :Artwork .


###  http://neo4j.com/voc/art#worksWith
:worksWith rdf:type owl:ObjectProperty ;
           rdfs:comment "represents some form of profesional relationship between two Persons" ;
           rdfs:range <https://schema.org/Person> ;
           rdfs:domain <https://schema.org/Person> .


#################################################################
#    Classes
#################################################################

###  http://neo4j.com/voc/art#Artist
:Artist rdf:type owl:Class ;
        rdfs:subClassOf <https://schema.org/Person> ;
        rdfs:comment "a creator of artworks" .


###  http://neo4j.com/voc/art#Artwork
:Artwork rdf:type owl:Class ;
         rdfs:subClassOf <https://schema.org/CreativeWork> ;
         rdfs:comment "an artistic creation" .


###  Generated by the OWL API (version 4.5.29.2024-05-13T12:11:03Z) https://github.com/owlcs/owlapi
